4. 
(1) 将生成式写成联立方程为： 
$$
\begin{array}{lcl}
S=baA+B\ \ \ \ \ \ \ \ \ \ \ (1)\\
A=aS+bB\ \ \ \ \ \ \ \ \ \ \ (2)\\
B=b+bC\ \ \ \ \ \ \ \ \ \ \ \ \ \ (3)\\
C=cB+d\ \ \ \ \ \ \ \ \ \ \ \ \ (4)\\
\end{array}
$$
将（4）代入（3）得：
$$
B=b+b(cB+d)=bcB+bd+b=(bc)^{*}(bd+b)\ \ \ \ \ \ \ \ \ \ \ \ \ \ \ \ (5)
$$
将（2）（5）代入（1）得：
$$
\begin{align}
S&=ba(aS+b(bc)^{*}(bd+b))+(bc)^{*}(bd+b)\\
&=baaS+bab(bc)^{*}(bd+b)+(bc)^{*}(bd+b)\\
&=(baa)^{*}(bab+\varepsilon)(bc)^{*}(bd+b)\\
\end{align}
$$
(2) 将生成式写成联立方程为：
$$
\begin{array}{lcl}
S=aA+B\ \ \ \ \ \ \ \ \ \ \ \ \ (1)\\
A=bB+cC\ \ \ \ \ \ \ \ \ \ \ (2)\\
B=a+bB\ \ \ \ \ \ \ \ \ \ \ \ \ (3)\\
C=D+abB\ \ \ \ \ \ \ \ \ \ (4)\\
D=d\ \ \ \ \ \ \ \ \ \ \ \ \ \ \ \ \ \ \ \ \ \ (5)\\
\end{array}
$$
由（3）得：
$$
B=b^{*}a \ \ \ \ \ \ \ \ \ \ \ (6)
$$
将（5）（6）代入（4）得：
$$
C=d+abb^{*}a=d+ab^{+}a\ \ \ \ \ \ \ \ \ \ \ (7)
$$
将（6）（7）代入（2）得：
$$
A=b^{+}a+c(d+ab^{+}a)\ \ \ \ \ \ \ \ \ \ \ (8)
$$
将（6）（8）代入（1）得：
$$
\begin{align}
S&=a(b^{+}a+c(d+ab^{+}a))+b^{*}a\\
&=ab^{+}a+acd+acab^{+}a+b^{*}a\\
\end{align}
$$

5. 
(2) 右线性文法 $G=(\{S\},\{a,b\},P,S)$，其中生成式 P 如下：
$$
S\rightarrow aS\ \ \ \ \ \ \ \ \ S\rightarrow bS\ \ \ \ \ \ \ \ \ S\rightarrow abb
$$
(4)右线性文法 $G=(\{S,A,B,C\},\{a,b\},P,S)$，其中生成式 P 如下：
$$
\begin{array}{lcl}
S\rightarrow aS|bS|aaA|bbB\\
A\rightarrow aA|bA|bbC\\
B\rightarrow aB|bB|aaC\\
C\rightarrow aC|bC|\varepsilon\\
\end{array}
$$
